wip

src/Thread.v
@@ -44,68 +44,84 @@ Local Open Scope itree_scope.
 Local Open Scope monad_scope.
 (* Local Open Scope monad_scope. *)
 
-Module Thread (Arch : Arch).
-  Definition mem_location := nat.
+Definition instruction_id_t := id_t.
 
-  Record mem_slc : Type :=
-    mk_mem_slc { addr : mem_location;
-                 size: nat (* in bytes *) }.
-  Definition mem_slc_val := nat.
-
+Module Denote (Arc : ArcSig).
   Definition mem_read_id_t := id_t.
   Record mem_read : Type :=
     mk_mem_read { read_id : mem_read_id_t;
-                  read_fp : mem_slc;
-                  read_kind : Arch.InsSem.mem_read_kind }.
+                  read_fp : Arc.mem_slc;
+                  read_kind : Arc.InsSem.mem_read_kind }.
 
   Definition mem_write_id_t := id_t.
   Record mem_write : Type :=
     mk_mem_write { write_id : mem_write_id_t;
-                   write_fp : mem_slc;
-                   write_kind : Arch.InsSem.mem_read_kind }.
+                   write_fp : Arc.mem_slc;
+                   write_kind : Arc.InsSem.mem_read_kind }.
 
-  Definition instruction_id_t := id_t.
 
-  Variant ITEThread : Type -> Type :=
-  | ITEFetch : mem_location -> ITEThread nat
-  | ITEDecode : nat -> ITEThread Arch.InsSem.ast
-  | ITENextLocs : mem_location -> Arch.InsSem.ast -> ITEThread (list mem_location).
+  Variant threadE : Type -> Type :=
+  | ThEInsFetch : Arc.InsSem.pc_t -> threadE Arc.InsSem.machine_code
+  | ThEInsDecode : Arc.InsSem.machine_code -> threadE Arc.InsSem.ast
+  | ThEInsNextLocs : Arc.InsSem.pc_t -> Arc.InsSem.ast ->
+                     threadE (list (instruction_id_t * Arc.InsSem.pc_t)).
+  (* | ThEInsSem : forall A, Arc.InsSem.E A -> threadE A. *)
+  (* Arguments ThEInsSem {A}. *)
 
-  Definition new_instruction {E} `{ITEThread -< E} `{Arch.InsSem.E -< E}
-    : ktree (nondet_schedulerE mem_location +' E) mem_location unit :=
-    fun loc =>
-      mem_val <- trigger (ITEFetch loc)
-      ;; ast <- trigger (ITEDecode mem_val)
-      ;; next_locs <- trigger (ITENextLocs loc ast)
-      ;; ITree.iter (fun locs =>
-                       match locs with
+  Context {E: Type -> Type}.
+  Context `{wrapE threadE instruction_id_t -< E}.
+  Context `{wrapE Arc.InsSem.E instruction_id_t -< E}.
+
+  Definition SE := nondet_schedulerE (instruction_id_t * Arc.InsSem.pc_t) +' E.
+
+  (* Definition handle_regE {E} *)
+  (*   : wrapE Arc.InsSem.regE instruction_id_t ~> itree E := *)
+  (*   fun _ e => *)
+  (*     let '(Wrap e iid) := e in *)
+  (*     match e with *)
+  (*     | Arc.InsSem.RegERead rslc => *)
+
+  (*       Ret (read_reg_slc rslc iid s) *)
+  (*     | Arc.InsSem.RegEWrite rslc rval => Ret (write_reg_slc rslc rval iid s, tt) *)
+  (*     end. *)
+
+  Definition new_instruction
+    : ktree SE (instruction_id_t * Arc.InsSem.pc_t) Types.result :=
+    fun '(id, loc) =>
+      mem_val <- trigger (Wrap (ThEInsFetch loc) id)
+      ;; ast <- trigger (Wrap (ThEInsDecode mem_val) id)
+      ;; next_ins <- trigger (Wrap (ThEInsNextLocs loc ast) id)
+      ;; ITree.iter (fun next_ins =>
+                       match next_ins with
                        | [] => ret (inr tt)
-                       | l::locs => trigger (Spawn l)
-                                  ;; ret (inl locs)
-                       end) next_locs
-      ;; resum_it unit (Arch.InsSem.denote ast).
+                       | (id, loc)::next_ins => trigger (Spawn (id, loc))
+                                              ;; ret (inl next_ins)
+                       end) next_ins
+      ;; resum_it _ (translate (fun _ e => Wrap e id) (Arc.InsSem.denote ast)
+                    ;; ret Accept).
 
-  Definition denote {E} `{ITEThread -< E} `{Arch.InsSem.E -< E}
-    : ktree (nondet_schedulerE mem_location +' E) mem_location unit :=
-    fun loc => nondet_scheduler new_instruction [new_instruction loc].
+  Definition denote
+    : ktree SE (instruction_id_t * Arc.InsSem.pc_t) Types.result :=
+    fun '(id, loc) => nondet_scheduler new_instruction [new_instruction (id, loc)].
+End Denote.
 
+(*******************************************************************************)
 
-
-
-
+Module State(Arc : ArcSig).
+  Module DenoteA := Denote Arc.
 
   Record mem_reads :=
-    mk_mem_reads { mr_footprint : mem_slc;
-                   mr_reads : list mem_read;
-                   mr_unsat_slcs : mem_read_id_t -> option (list mem_slc);
+    mk_mem_reads { mr_footprint : Arc.mem_slc;
+                   mr_reads : list DenoteA.mem_read;
+                   mr_unsat_slcs : DenoteA.mem_read_id_t -> option (list Arc.mem_slc);
                    mr_reads_from :
-                     mem_read_id_t -> option (list (instruction_id_t * mem_write_id_t * mem_slc)) }.
+                     DenoteA.mem_read_id_t -> option (list (instruction_id_t * DenoteA.mem_write_id_t * Arc.mem_slc)) }.
 
   Record mem_writes :=
-    mk_mem_writes { mw_footprint : mem_slc;
-                    mw_writes : list mem_write;
-                    mw_write_val : mem_write_id_t -> option mem_slc_val;
-                    mw_has_propagated : mem_write_id_t -> option bool;
+    mk_mem_writes { mw_footprint : Arc.mem_slc;
+                    mw_writes : list DenoteA.mem_write;
+                    mw_write_val : DenoteA.mem_write_id_t -> option Arc.mem_slc_val;
+                    mw_has_propagated : DenoteA.mem_write_id_t -> option bool;
                     mw_committed : bool }.
 
   Variant instruction_exec_state : Type :=
@@ -118,21 +134,17 @@ Module Thread (Arch : Arch).
   Record fetched_instruction_state :=
     mk_fetched_instruction_state {
         ins_id : instruction_id_t;
-        ins_loc : mem_location; (*: record fetched address :*)
-        ins_ast : Arch.InsSem.ast;
+        ins_loc : Arc.mem_loc; (*: record fetched address :*)
         (* statically analysed data about the instruction*)
-        ins_kind: Arch.instruction_kind;
-
-        (* ins_initial_semantics_state: instruction_semantics_state; *)
-        ins_sem: Arch.InsSem.sem_t;
+        ins_kind: Arc.instruction_kind;
 
         (*: The input registers, for ease of dependency calculation :*)
-        ins_regs_in : ListSet.set Arch.InsSem.reg_slc;
+        ins_regs_in : ListSet.set Arc.InsSem.reg_slc;
 
         (*: The input registers that feed into a memory access address :*)
-        ins_regs_feeding_address: ListSet.set Arch.InsSem.reg_slc;
+        ins_regs_feeding_address: ListSet.set Arc.InsSem.reg_slc;
         (*: The output registers, for ease of dependency calculation *)
-        ins_regs_out: ListSet.set Arch.InsSem.reg_slc;
+        ins_regs_out: ListSet.set Arc.InsSem.reg_slc;
 
         (* dynamic info *)
 
@@ -147,16 +159,17 @@ Module Thread (Arch : Arch).
 
         ins_exec_state: instruction_exec_state }.
 
-  Definition initial_fetched_instruction_state (loc : mem_location)
-             (ast : Arch.InsSem.ast)
+  Instance eta_fetched_instruction_state : Settable _ :=
+    settable! mk_fetched_instruction_state <ins_id; ins_loc; ins_kind; ins_regs_in; ins_regs_feeding_address; ins_regs_out; ins_mem_reads; ins_mem_writes; ins_finished; ins_exec_state>.
+
+  Definition initial_fetched_instruction_state (loc : Arc.mem_loc)
+             (ast : Arc.InsSem.ast)
     : fetched_instruction_state :=
-    let '(regs_in, regs_feeding_address, regs_out) := Arch.InsSem.regs_from_ast ast in
+    let '(regs_in, regs_feeding_address, regs_out) := Arc.InsSem.regs_from_ast ast in
     (* instruction_state: *)
     {| ins_id := 0; (* FIXME: get fresh id *)
        ins_loc := loc;
-       ins_ast := ast;
-       ins_kind := (Arch.instruction_kind_from_ast ast);
-       ins_sem := Arch.InsSem.denote ast;
+       ins_kind := (Arc.instruction_kind_from_ast ast);
        ins_regs_in := regs_in;
        ins_regs_feeding_address := regs_feeding_address;
        ins_regs_out := regs_out;
@@ -165,33 +178,56 @@ Module Thread (Arch : Arch).
        ins_finished := false;
        ins_exec_state := IESFetched |}.
 
-  Instance eta_fetched_instruction_state : Settable _ :=
-    settable! mk_fetched_instruction_state <ins_id; ins_loc; ins_ast; ins_kind; ins_sem; ins_regs_in; ins_regs_feeding_address; ins_regs_out; ins_mem_reads; ins_mem_writes; ins_finished; ins_exec_state>.
-
   Variant instruction_state :=
-  | ISUnfetched : mem_location -> instruction_state
+  | ISUnfetched : Arc.mem_loc -> instruction_state
   | ISFetched : fetched_instruction_state -> instruction_state.
 
-  Definition thread_id_t := id_t.
+  Record state :=
+    mk_state {
+        next_iid : instruction_id_t;
+        instruction_tree : tree instruction_state }.
 
-  Record thread_state :=
-    mk_thread_state {
-        thr_id : thread_id_t;
-        thr_instruction_tree : tree instruction_state }.
+  Instance eta_state : Settable _ :=
+    settable! mk_state <next_iid; instruction_tree>.
 
-  Definition initial_thread_state (id : thread_id_t) (loc : mem_location)
-    : thread_state :=
-    {| thr_id := id;
-       thr_instruction_tree := Tree (ISUnfetched loc) [] |}.
+  Definition initial_state (loc : Arc.mem_loc)
+    : state :=
+    {| next_iid := 0;
+       instruction_tree := Tree (ISUnfetched loc) [] |}.
 
-  Definition read_reg_slc (rslc : Arch.InsSem.reg_slc) (i : instruction_state) (s : thread_state)
-    : (instruction_state * thread_state * Arch.InsSem.reg_val) :=
+  Definition read_reg_slc (rslc : Arc.InsSem.reg_slc) (iid : instruction_id_t) (s : state)
+    : (state * Arc.InsSem.reg_val) :=
     (* FIXME: *)
-    (i, s, 0%N).
+    (s, 0%N).
 
-  Definition write_reg_slc (rslc : Arch.InsSem.reg_slc) (val : Arch.InsSem.reg_val)
-             (i : instruction_state) (s : thread_state)
-    : (instruction_state *thread_state) :=
+  Definition write_reg_slc (rslc : Arc.InsSem.reg_slc) (val : Arc.InsSem.reg_val)
+             (iid : instruction_id_t) (s : state)
+    : state :=
     (* FIXME: *)
-    (i, s).
-End Thread.
+    s.
+
+
+  Definition handle_regE {E} : wrapE Arc.InsSem.regE instruction_id_t ~> stateT state (itree E) :=
+    fun _ e s =>
+      let '(Wrap e iid) := e in
+      match e with
+      | Arc.InsSem.RegERead rslc => Ret (read_reg_slc rslc iid s)
+      | Arc.InsSem.RegEWrite rslc rval => Ret (write_reg_slc rslc rval iid s, tt)
+      end.
+
+  (* Definition handle_thread {E} : Arc.InsSem.E ~> stateT thread_state (itree E) :=. *)
+
+  (* Definition handle_thread {E} : threadE ~> stateT thread_state (itree E) := *)
+  (*   fun _ e thread_state => *)
+  (*     match e with *)
+  (*     | *)
+
+  (* (* SAZ: I think that all of these [run_foo] functions should be renamed *)
+  (*    [interp_foo].  That would be more consistent with the idea that *)
+  (*    we define semantics by nested interpretation.  Also, it seems a bit *)
+  (*    strange to define [interp_map] in terms of [interp_state]. *)
+  (* *) *)
+  (* Definition interp_map {E d} : itree (mapE d +' E) ~> stateT map (itree E) := *)
+  (*   interp_state (case_ handle_map pure_state). *)
+
+End State.
