src/Utils.v
@@ -28,11 +28,14 @@ Local Open Scope list.
 Local Open Scope itree_scope.
 (* Local Open Scope monad_scope. *)
 
-Notation " x '|>' f " := (f x)
+(* The [sum1] types with automatic application of commutativity and
+   associativity are prone to infinite instance resolution loops.
+   This bounds the instance search depth: *)
+Typeclasses eauto := 5.
+
+Notation " x '$>' f " := (f x)
   (at level 40, left associativity, only parsing).
 
-Definition resum_it {E F} `{E -< F} : itree E ~> itree F :=
-  fun _ it => interp (fun _ e => trigger e) it.
 
 Fixpoint list_replace_nth {T} (n : nat) (x : T) (l : list T) : list T :=
   match n, l with
@@ -41,6 +44,7 @@ Fixpoint list_replace_nth {T} (n : nat) (x : T) (l : list T) : list T :=
   | _, _ => nil
   end.
 
+
 Fixpoint list_remove_nth {T} (n : nat) (l : list T) : list T :=
   match n, l with
   | O, _::t => t
@@ -48,39 +52,70 @@ Fixpoint list_remove_nth {T} (n : nat) (l : list T) : list T :=
   | _, _ => nil
   end.
 
+
+Inductive tree (T : Type) : Type :=
+| Tree : T -> list (tree T) -> tree T.
+Arguments Tree {T}.
+
+Fixpoint tree_map_with_context {T Y : Type}
+         (f : list T -> T -> list (tree T) -> Y) (pref : list T) (t : tree T)
+  : tree Y :=
+  let '(Tree x ts) := t in
+  Tree (f pref x ts) (List.map (tree_map_with_context f (x::pref)) ts).
+
+Definition id_t := nat.
+
+
+
+Definition resum_it {E F} `{E -< F} : itree E ~> itree F :=
+  fun _ it => interp (fun _ e => trigger e) it.
+
+Variant wrapE E T : Type -> Type :=
+| Wrap : forall A, E A -> T -> wrapE E T A.
+Arguments Wrap {E T A}.
+
+Definition wrap_it {T E F} `{wrapE E T -< F} (d : T) : itree E ~> itree F :=
+  fun _ it => interp (fun _ e => trigger (Wrap e d)) it.
+
+
 Variant nondet_schedulerE (S : Type) : Type -> Type :=
 | NondetFin : nat -> nondet_schedulerE S nat
 | Spawn : S -> nondet_schedulerE S unit.
 Arguments NondetFin {S}.
 Arguments Spawn {S}.
 
-CoFixpoint nondet_scheduler {E S}
-           (spawn : ktree (nondet_schedulerE S +' E) S unit)
-           (its : list (itree (nondet_schedulerE S +' E) unit))
-  : itree (nondet_schedulerE S +' E) unit :=
+CoFixpoint nondet_scheduler {E S IR R}
+           (spawn : ktree (nondet_schedulerE S +' E) S IR)
+           (fold_results : R -> IR -> R)
+           (acc_result : R)
+           (its : list (itree (nondet_schedulerE S +' E) IR))
+  : itree (nondet_schedulerE S +' E) R :=
   match its with
-  | [] => Ret tt
+  | [] => Ret acc_result
   | _ =>
     n <- trigger (NondetFin (List.length its))
     ;; match List.nth_error its n with
        | Some it =>
          match observe it with
-         | RetF _ => Tau (nondet_scheduler spawn (list_remove_nth n its))
-         | TauF it => Tau (nondet_scheduler spawn (list_replace_nth n it its))
+         | RetF r =>
+           let acc_result := fold_results acc_result r in
+           Tau (nondet_scheduler spawn fold_results acc_result (list_remove_nth n its))
+         | TauF it =>
+           Tau (nondet_scheduler spawn fold_results acc_result (list_replace_nth n it its))
          | @VisF _ _ _ X o k =>
            match o with
            | inl1 o' =>
              match o' in nondet_schedulerE _ Y
-                   return X = Y -> itree (nondet_schedulerE S +' E) unit with
+                   return X = Y -> itree (nondet_schedulerE S +' E) R with
              | Spawn s =>
                fun pf =>
                  let it := k (eq_rect_r (fun T => T) tt pf) in
-                 Tau (nondet_scheduler spawn (spawn s::list_replace_nth n it its))
+                 Tau (nondet_scheduler spawn fold_results acc_result(spawn s::list_replace_nth n it its))
              | _ => fun _ =>
-                     Vis o (fun x => nondet_scheduler spawn (list_replace_nth n (k x) its))
+                     Vis o (fun x => nondet_scheduler spawn fold_results acc_result (list_replace_nth n (k x) its))
              end eq_refl
            | inr1 _ =>
-             Vis o (fun x => nondet_scheduler spawn (list_replace_nth n (k x) its))
+             Vis o (fun x => nondet_scheduler spawn fold_results acc_result (list_replace_nth n (k x) its))
            end
          end
        | None => ITree.spin (* catch fire *)
