src/Storage.v
@@ -1,0 +1,40 @@
+From Coq Require Import
+     Arith.PeanoNat
+     NArith.NArith
+     Lists.List
+     Lists.ListSet
+     (* Strings.String *)
+     Morphisms
+     Setoid
+     RelationClasses .
+
+From ExtLib Require Import
+     Structures.Monads
+     Data.Monads.ListMonad.
+(*      Data.String *)
+(*      Structures.Traversable *)
+(*      Data.List. *)
+
+From RecordUpdate Require Import RecordSet.
+
+Import ListMonad.
+Import Monads.
+Import MonadNotation.
+Import ListNotations.
+
+Require Import Utils.
+Require Import Types.
+Require Import Thread.
+
+Local Open Scope list.
+Local Open Scope itree_scope.
+Local Open Scope monad_scope.
+(* Local Open Scope monad_scope. *)
+
+Module State (Arc : ArcSig).
+  Record state := mk_state { mem : Arc.mem_loc -> option Arc.mem_slc_val }.
+  Instance eta_state : Settable _ := settable! mk_state <mem>.
+
+  Definition initial_state (mem : Arc.mem_loc -> option Arc.mem_slc_val) : state :=
+    {| mem := mem |}.
+End State.
