src/System.v
@@ -1,0 +1,150 @@
+From Coq Require Import
+     Arith.PeanoNat
+     NArith.NArith
+     Lists.List
+     Lists.ListSet
+     (* Strings.String *)
+     Morphisms
+     Setoid
+     RelationClasses .
+
+From ExtLib Require Import
+     Structures.Monads
+     Data.Monads.ListMonad.
+(*      Data.String *)
+(*      Structures.Traversable *)
+(*      Data.List. *)
+
+From ITree Require Import
+     ITree
+     ITreeFacts
+     Events.MapDefault
+     Events.StateFacts
+     Events.Nondeterminism.
+
+(* The [sum1] types with automatic application of commutativity and
+   associativity are prone to infinite instance resolution loops.
+   This bounds the instance search depth: *)
+Typeclasses eauto := 5.
+
+From RecordUpdate Require Import RecordSet.
+
+Import ListMonad.
+Import ITreeNotations.
+Import Monads.
+Import MonadNotation.
+Import ListNotations.
+Import RecordSetNotations.
+
+Require Import Utils.
+Require Import Types.
+Require Import Thread.
+Require Import Storage.
+
+Local Open Scope list.
+Local Open Scope itree_scope.
+Local Open Scope monad_scope.
+
+(* Local Open Scope monad_scope. *)
+
+Module System (Arc : ArcSig).
+  Module ThrDenote := Thread.Denote Arc.
+  Definition thread_id_t := Utils.id_t.
+
+  Definition denote {E}
+             `{wrapE ThrDenote.SE thread_id_t -< E}
+             (entry_locs : list nat)
+    : itree (nondet_schedulerE unit +' E) unit :=
+    List.length entry_locs
+    $> List.seq 0
+    $> List.combine entry_locs
+    $> List.map (fun '(eloc, tid) => wrap_it tid _ (ThrDenote.denote (0, eloc)))
+    $> nondet_scheduler (fun tt => ITree.spin).
+       (* The spin is unreachable.
+          TODO: do we want to support spawning of new threads?
+          Probably not. *)
+
+
+
+
+  Module ThrState := Thread.State Arc.
+  Module StoState := Storage.State Arc.
+
+  Record state :=
+    mk_state {
+        storage : StoState.state;
+        (* thread-tid is in index tid *)
+        threads : list ThrState.state }.
+
+  Instance eta_state : Settable _ :=
+    settable! mk_state <storage; threads>.
+
+  Definition initial_state (mem : Arc.mem_loc -> option Arc.mem_slc_val) (entry_locs : list Arc.mem_loc)
+    : state :=
+    {| storage := StoState.initial_state mem;
+       threads := List.map ThrState.initial_state entry_locs |}.
+
+  Definition handle_thr_regE {E}
+    : wrapE (wrapE Arc.InsSem.regE Thread.instruction_id_t) thread_id_t ~> stateT state (itree E) :=
+    fun _ e s =>
+      let '(Wrap e tid) := e in
+      match List.nth_error s.(threads) tid with
+      | Some thr_state =>
+        '(thr_state, a) <- ThrState.handle_regE _ e thr_state
+        ;; let ts := list_replace_nth tid thr_state s.(threads) in
+           Ret (s <| threads := ts |>, a)
+      | None => ITree.spin (* Unreachable *)
+      end.
+
+  Definition handle_thr_memE {E}
+    : wrapE (wrapE Arc.InsSem.memE Thread.instruction_id_t) thread_id_t ~> stateT state (itree E) :=
+    fun _ e s =>
+      let '(Wrap e tid) := e in
+      match List.nth_error s.(threads) tid with
+      | Some thr_state =>
+        '(thr_state, a) <- ThrState.handle_memE _ e thr_state
+        ;; let ts := list_replace_nth tid thr_state s.(threads) in
+           Ret (s <| threads := ts |>, a)
+      | None => ITree.spin (* Unreachable *)
+      end.
+
+  Definition handle_threadE {E}
+    : wrapE (wrapE ThrDenote.threadE Thread.instruction_id_t) thread_id_t ~> stateT state (itree E) :=
+    fun _ e s =>
+      let '(Wrap e tid) := e in
+      match List.nth_error s.(threads) tid with
+      | Some thr_state =>
+        let '(Wrap e iid) := e in
+        match e with
+        | ThEFetch loc => Ret(s, 0%N) (* FIXME: *)
+        | ThEDecode code => Ret(s, Arc.InsSem.decode code)
+        | ThENextLocs loc ast =>
+          let next_pcs := Arc.InsSem.next_pc loc ast in
+          let iids := List.seq thr_state.(next_iid) (List.length next_pcs) in
+          let thr_state := thr_state <| next_iid := thr_state.(next_iid) + (List.length next_pcs) |> in
+          let ts := list_replace_nth tid thr_state s.(threads) in
+          Rest(s <| thread := ts |>, list.compose iids next_pcs)
+        end
+      | None => ITree.spin (* Unreachable *)
+      end.
+
+
+
+
+
+
+
+
+      Definition interp_system {E}
+                 (it : itree (systemE +' E) unit)
+        : system_state -> itree E (system_state * unit) :=
+        let h := bimap h_reg (bimap h_memory (id_ _)) in
+        let it := interp h it in
+        fun s => interp_map (interp_map t' regs) mem.
+
+
+      (** We can then define an evaluator for closed assembly programs by interpreting
+    both store and heap events into two instances of [mapE], and running them
+    both in the empty initial environments.  *)
+      Definition run_system (mem : nat -> option nat) (entry_locs : list nat) :=
+        interp_system (denote entry_locs) (initial_state mem entry_locs).
